added Positional wrappers for Associational operations, added correctness proof of

src/NewBaseSystem.v
@@ -418,7 +418,7 @@ Module B.
         nsatz.
       Qed. Hint Rewrite eval_carryterm using auto : push_basesystem_eval.
 
-      Definition carry_cps(w fw:Z) (p:list limb) {T} (f:list limb->T) :=
+      Definition carry_cps (w fw:Z) (p:list limb) {T} (f:list limb->T) :=
         flat_map_cps (carryterm_cps w fw) p f.
 
       Definition carry w fw p := carry_cps w fw p id.
@@ -595,13 +595,56 @@ Module B.
       Proof. cbv [carry_cps carry]; intros; eapply @eval_carry; eauto. Qed.
       Hint Rewrite @eval_carry : push_basesystem_eval.
 
-      (* TODO make a correctness proof for this *)
-      Definition chained_carries (p:list limb) (idxs : list nat)
-                 {T} (f:list limb->T) :=
-        fold_right_cps2 carry_cps p idxs f.
+      Definition chained_carries_cps {n} (p:tuple Z n) (idxs : list nat)
+                 {T} (f:tuple Z n->T) :=
+        to_associational_cps p
+          (fun P => fold_right_cps2 carry_cps P idxs
+            (fun R => from_associational_cps n R f)).
+      
+      Definition chained_carries {n} p idxs := @chained_carries_cps n p idxs _ id.
+      Lemma chained_carries_id {n} p idxs : forall {T} f,
+          @chained_carries_cps n p idxs T f = f (chained_carries p idxs).
+      Proof. cbv [chained_carries_cps chained_carries]; prove_id. Qed.
+      Hint Opaque chained_carries : uncps.
+      Hint Rewrite @chained_carries_id : uncps.
+
+      Lemma eval_chained_carries {n} (p:tuple Z n) idxs :
+        (forall i, In i idxs -> weight (S i) / weight i <> 0) ->
+        eval (chained_carries p idxs) = eval p.
+      Proof.
+        cbv [chained_carries chained_carries_cps]; intros;
+          autorewrite with uncps push_id.
+        apply fold_right_invariant; destruct n; prove_eval; auto.
+      Qed. Hint Rewrite @eval_chained_carries : push_basesystem_eval.
       End Carries.
+
+      Section Wrappers.
+        (* Simple wrappers for Associational definitions; convert to
+        associational, do the operation, convert back. *)
+
+        Definition add_cps {n} (p q : tuple Z n) {T} (f:tuple Z n->T) :=
+          to_associational_cps p
+            (fun P => to_associational_cps q
+              (fun Q => from_associational_cps n (P++Q) f)).
+
+        Definition mul_cps {n m} (p q : tuple Z n) {T} (f:tuple Z m->T) :=
+          to_associational_cps p
+            (fun P => to_associational_cps q
+              (fun Q => Associational.mul_cps P Q
+                (fun PQ => from_associational_cps m PQ f))).
+
+        Definition reduce_cps {m n} (s:Z) (c:list B.limb) (p : tuple Z m)
+                   {T} (f:tuple Z n->T) :=
+          to_associational_cps p
+            (fun P => Associational.reduce_cps s c P
+                (fun R => from_associational_cps n R f)).
+      End Wrappers.
     End Positional.
   End Positional.
+  Hint Unfold
+      Positional.add_cps 
+      Positional.mul_cps
+      Positional.reduce_cps.
   Hint Rewrite
       @Associational.carry_cps_id
       @Associational.carryterm_cps_id
@@ -613,6 +656,7 @@ Module B.
       @Positional.place_cps_id
       @Positional.add_to_nth_cps_id
       @Positional.to_associational_cps_id
+      @Positional.chained_carries_id
     : uncps.
   Hint Rewrite
       @Associational.eval_mul
@@ -624,6 +668,7 @@ Module B.
       @Positional.eval_carry
       @Positional.eval_from_associational
       @Positional.eval_add_to_nth
+      @Positional.eval_chained_carries
     using (omega || assumption) : push_basesystem_eval.
 End B.
   
@@ -635,7 +680,7 @@ Ltac basesystem_partial_evaluation_RHS :=
   let t0 := match goal with |- _ _ ?t => t end in
   let t := (eval cbv delta [
   (* this list must contain all definitions referenced by t that reference [Let_In], [runtime_add], or [runtime_mul] *)
-Positional.to_associational_cps Positional.to_associational Positional.eval Positional.zeros Positional.add_to_nth_cps Positional.add_to_nth Positional.place_cps Positional.place Positional.from_associational_cps Positional.from_associational Positional.carry_cps Positional.carry Positional.chained_carries
+Positional.to_associational_cps Positional.to_associational Positional.eval Positional.zeros Positional.add_to_nth_cps Positional.add_to_nth Positional.place_cps Positional.place Positional.from_associational_cps Positional.from_associational Positional.carry_cps Positional.carry Positional.chained_carries_cps Positional.chained_carries
 Associational.eval Associational.multerm Associational.mul_cps Associational.mul Associational.split_cps Associational.split Associational.reduce_cps Associational.reduce Associational.carryterm_cps Associational.carryterm Associational.carry_cps Associational.carry 
                  ] in t0) in
   let t := (eval pattern @runtime_mul in t) in
@@ -662,6 +707,10 @@ Ltac assert_preconditions :=
            unique assert (n <> 0%nat) by (cbv; congruence)
          | |- context [Positional.carry_cps?wt ?i] =>
            unique assert (wt (S i) / wt i <> 0) by (cbv; congruence)
+         | |- context [Positional.chained_carries_cps ?wt _ ?idxs] =>
+           unique assert (forall i, In i idxs -> wt (S i) / wt i <> 0)
+             by (clear; simpl;  intuition; subst_let; subst; cbv in *;
+                 congruence)
          | |- context [Associational.reduce_cps ?s _] =>
            unique assert (s <> 0) by (cbv; congruence)
          | |- context [Associational.reduce_cps ?s ?c] =>
@@ -716,13 +765,10 @@ Section Ops.
                  eval (add a b) = eval a  + eval b }.
   Proof.
     let x := constr:(fun wt a b =>
-        Positional.to_associational_cps (n := sz) wt a
-          (fun r => Positional.to_associational_cps (n := sz) wt b
-          (fun r0 => Positional.from_associational_cps wt sz (r ++ r0) id
-                    ))) in
+        Positional.add_cps (n := sz) wt a b id) in
     lift2_sig; eexists;
-    transitivity (Positional.eval wt (x wt a b));
-      [|assert_preconditions; autorewrite with uncps push_id push_basesystem_eval; reflexivity].
+    transitivity (Positional.eval wt (x wt a b)); autounfold;
+    [|assert_preconditions; autorewrite with uncps push_id push_basesystem_eval; reflexivity].
 
     apply f_equal.
     
@@ -738,20 +784,12 @@ Section Ops.
                  mod_eq m (eval (mul a b)) (eval a  * eval b)}.
   Proof.
     let x := constr:(fun w a b =>
-         Positional.to_associational_cps (n := sz) w a
-           (fun r => Positional.to_associational_cps (n := sz) w b
-           (fun r0 => Associational.mul_cps r r0
-           (fun r1 => Positional.from_associational_cps w sz2 r1
-           (fun r2 => Positional.to_associational_cps w r2
-           (fun r3 => Associational.reduce_cps s c r3       
-           (fun r4 => Positional.from_associational_cps w sz r4
-           (fun r5 => Positional.to_associational_cps w r5
-           (fun r6 => Positional.chained_carries(div:=div)(modulo:=modulo) w r6 (seq 0 sz)
-           (fun r13 => Positional.from_associational_cps w sz r13 id
-             )))))))))) in
+         Positional.mul_cps (n:=sz) (m:=sz2) w a b
+           (fun ab => Positional.reduce_cps (n:=sz) (m:=sz2) w s c ab
+           (fun r => Positional.chained_carries_cps (n:=sz) (div:=div)(modulo:=modulo) w r (seq 0 sz) id))) in
     lift2_sig; eexists;
-    transitivity (Positional.eval wt (x wt a b));
-    [|cbv [Positional.chained_carries fold_right_cps2 seq fold_right sz2 sz]; assert_preconditions; autorewrite with uncps push_id push_basesystem_eval; reflexivity].
+    transitivity (Positional.eval wt (x wt a b)); autounfold;
+      [|assert_preconditions; autorewrite with uncps push_id push_basesystem_eval; reflexivity].
 
     cbv [mod_eq].
     apply f_equal2; [|reflexivity].
